src/Eqvivalence/FsBs/F1GiveNames.v
@@ -648,41 +648,6 @@ Fixpoint give_pats
 
 
 
-Fixpoint give_val
-    (v : Val)
-    : Value
-    :=
-  match v with
-
-  | Syntax.VNil =>
-    VNil
-
-  | Syntax.VLit l =>
-    VLit
-      (convert_lit l)
-
-  | Syntax.VCons v₁ v₂ =>
-    VCons
-      (give_val v₁)
-      (give_val v₂)
-
-  | Syntax.VTuple vs =>
-    VTuple
-      (map give_val vs)
-
-  | Syntax.VMap vvs =>
-    VMap
-      (map (fun '(x, y) => (give_val x, give_val y)) vvs)
-
-  | _ => VNil
-
-  end.
-
-
-
-
-
-
 
 
 
@@ -823,6 +788,44 @@ with give_eexp
     ELetRec
       (give_ext_noid give_exp (count_binds_exp ᵇe + n) os)
       (give_exp n ᵇe) *)
+
+  end.
+
+
+
+
+
+
+Fixpoint give_val
+    (v : Val)
+    : Value
+    :=
+  match v with
+
+  | Syntax.VNil =>
+    VNil
+
+  | Syntax.VLit l =>
+    VLit
+      (convert_lit l)
+
+  | Syntax.VCons v₁ v₂ =>
+    VCons
+      (give_val v₁)
+      (give_val v₂)
+
+  | Syntax.VTuple vs =>
+    VTuple
+      (map give_val vs)
+
+  | Syntax.VMap vvs =>
+    VMap
+      (map (fun '(x, y) => (give_val x, give_val y)) vvs)
+
+  (* TMP *)
+  | Syntax.VClos _ _ _ _ => VNil
+
+  | _ => VNil
 
   end.
 
@@ -1137,6 +1140,650 @@ End TestSuccess.
 From CoreErlang.Eqvivalence Require Export BX3Tactics.
 
 Section FsBs.
+
+
+
+Lemma destruct_vnil :
+  forall r,
+      ⟨ [], ˝VNil ⟩ -->* (to_redex r)
+  ->  r = inl [VNil].
+Proof.
+  itr.
+  des - r as [vs | q]; smp *.
+  * ivc - H as [k [_ H1]].
+    ivc - H1.
+    ivc - H.
+    ivc - H0.
+    trv.
+    ivc - H.
+  * ivc - H as [k [_ H1]].
+    ivc - H1.
+    ivc - H.
+    ivc - H0.
+    ivc - H.
+Qed.
+
+
+
+Lemma destruct_vlit :
+  forall l r,
+      ⟨ [], ˝(VLit l) ⟩ -->* (to_redex r)
+  ->  r = inl [VLit l].
+Proof.
+  itr.
+  des - r as [vs | q]; smp *.
+  * ivc - H as [k [_ H1]].
+    ivc - H1.
+    ivc - H.
+    ivc - H0.
+    trv.
+    ivc - H.
+  * ivc - H as [k [_ H1]].
+    ivc - H1.
+    ivc - H.
+    ivc - H0.
+    ivc - H.
+Qed.
+
+
+
+Lemma destruct_vvar :
+  forall x r,
+      ⟨ [], ˝(VVar x) ⟩ -->* (to_redex r)
+  ->  False.
+Proof.
+  itr.
+  des - r as [vs | q]; smp *.
+  * ivc - H as [k [_ H1]].
+    ivc - H1.
+    ivc - H.
+    ivc - H0.
+    ivc - H3.
+    ivc - H1.
+    ivc - H.
+  * ivc - H as [k [_ H1]].
+    ivc - H1.
+    ivc - H.
+    ivc - H0.
+    ivc - H.
+Qed.
+
+
+
+Lemma destruct_vfunid :
+  forall f r,
+      ⟨ [], ˝(VFunId f) ⟩ -->* (to_redex r)
+  ->  False.
+Proof.
+  itr.
+  des - r as [vs | q]; smp *.
+  * ivc - H as [k [_ H1]].
+    ivc - H1.
+    ivc - H.
+    ivc - H0.
+    ivc - H3.
+    ivc - H1.
+    ivc - H.
+  * ivc - H as [k [_ H1]].
+    ivc - H1.
+    ivc - H.
+    ivc - H0.
+    ivc - H.
+Qed.
+
+
+
+Lemma destruct_vcons :
+  forall v1 v2 r,
+      ⟨ [], ˝(VCons v1 v2) ⟩ -->* (to_redex r)
+  ->  r = inl [VCons v1 v2].
+Proof.
+  itr.
+  des - r as [vs | q]; smp *.
+  * ivc - H as [k [_ H1]].
+    ivc - H1.
+    ivc - H.
+    ivc - H0.
+    trv.
+    ivc - H.
+  * ivc - H as [k [_ H1]].
+    ivc - H1.
+    ivc - H.
+    ivc - H0.
+    ivc - H.
+Qed.
+
+
+
+Lemma destruct_vtuple :
+  forall vl r,
+      ⟨ [], ˝(VTuple vl) ⟩ -->* (to_redex r)
+  ->  r = inl [VTuple vl].
+Proof.
+  itr.
+  des - r as [vs | q]; smp *.
+  * ivc - H as [k [_ H1]].
+    ivc - H1.
+    ivc - H.
+    ivc - H0.
+    trv.
+    ivc - H.
+  * ivc - H as [k [_ H1]].
+    ivc - H1.
+    ivc - H.
+    ivc - H0.
+    ivc - H.
+Qed.
+
+
+
+Lemma destruct_vmap :
+  forall vvl r,
+      ⟨ [], ˝(VMap vvl) ⟩ -->* (to_redex r)
+  ->  r = inl [VMap vvl].
+Proof.
+  itr.
+  des - r as [vs | q]; smp *.
+  * ivc - H as [k [_ H1]].
+    ivc - H1.
+    ivc - H.
+    ivc - H0.
+    trv.
+    ivc - H.
+  * ivc - H as [k [_ H1]].
+    ivc - H1.
+    ivc - H.
+    ivc - H0.
+    ivc - H.
+Qed.
+
+
+
+Lemma destruct_vclos :
+  forall os id xs e r,
+      ⟨ [], ˝(VClos os id xs e) ⟩ -->* (to_redex r)
+  ->  r = inl [VClos os id xs e].
+Proof.
+  itr.
+  des - r as [vs | q]; smp *.
+  * ivc - H as [k [_ H1]].
+    ivc - H1.
+    ivc - H.
+    ivc - H0.
+    trv.
+    ivc - H.
+  * ivc - H as [k [_ H1]].
+    ivc - H1.
+    ivc - H.
+    ivc - H0.
+    ivc - H.
+Qed.
+
+
+Axiom no_pid :
+  forall v,
+    v <> VPid.
+
+Axiom no_reference :
+  forall e,
+  (forall x, e <> give_names (˝VVar x))
+  /\
+  (forall f, e <> give_names (˝VFunId f)).
+
+
+
+Theorem destruct_value :
+  forall v r,
+      ⟨ [], ˝v ⟩ -->* (to_redex r)
+  ->  r = inl [v].
+Proof.
+  itr.
+  des - v.
+  bpp - destruct_vnil.
+  bpp - destruct_vlit.
+  pse - no_pid. con.
+  bpp - destruct_vcons.
+  bpp - destruct_vtuple.
+  bpp - destruct_vmap.
+  app - destruct_vvar in H. ivs - H.
+  app - destruct_vfunid in H. ivs - H.
+  bpp - destruct_vclos.
+Qed.
+
+
+
+
+
+Import BigStep.
+Definition eval_expr_simpl
+    (e : Expression)
+    (r : (ValueSequence + Exception))
+    : Prop
+    := 
+    forall id1, exists id2,
+        eval_expr [] [] "" id1 e [] id2 r [].
+
+
+Import SubstSemantics.
+
+Theorem value_to_value :
+  forall v,
+    eval_expr_simpl (give_names (˝v)) (give_result (inl [v])).
+Proof.
+  itr.
+  smp.
+  ind ~ ind_fs_val - v.
+  * sbn. eei. cns.
+  * sbn. eei. cns.
+  * pse - no_pid. eei. con.
+  * pse - no_reference: (give_names (˝ VVar x)).
+    des - H as [H _].
+    spe - H: x.
+    con.
+  * pse - no_reference: (give_names (˝ VFunId f)).
+    des - H as [_ H].
+    spe - H: f.
+    con.
+  * sbn *.
+    rem - v1' v2' v1'' v2'' as H1 H2 H3 H4 / H1 H2 H3 H4:
+          (give_vval 0 v1)
+          (give_vval 0 v2)
+          (give_val v1)
+          (give_val v2).
+    unfold eval_expr_simpl.
+    itr.
+    spe - IHv2: id1.
+    des - IHv2 as [id2 IHv2].
+    spe - IHv1: id2.
+    des - IHv1 as [id3 IHv1].
+    exi - id3.
+    ens.
+    exa - IHv2.
+    exa - IHv1.
+  * sbn *.
+    admit.
+  * admit.
+  * admit.
+Admitted.
+
+
+
+(* Theorem if_valseq_than_value :
+  forall Fs e vs,
+      ⟨ Fs, e ⟩ -->* (RValSeq vs)
+  ->  exists vs',
+        ⟨ Fs, RValSeq vs' ⟩ -->* (RValSeq vs).
+Proof.
+  itr.
+  ivc - H as [k [H1 H2]].
+  ivs - H2.
+  * exi - vs.
+    open.
+    step.
+  * ivs - H.
+    - exi - [v].
+      open.
+      exa - H0.
+    -  *)
+
+
+
+Lemma destruct_econs :
+  forall e1 e2 r,
+      ((exists v1 v2,
+          r = inl [VCons v1 v2]
+      /\  ⟨ [], RExp e1 ⟩ -->* (to_redex (inl [v1]))
+      /\  ⟨ [], RExp e2 ⟩ -->* (to_redex (inl [v2])))
+  \/  (exists q1 v2,
+          r = inr q1
+      /\  ⟨ [], RExp e1 ⟩ -->* (to_redex (inr q1))
+      /\  ⟨ [], RExp e2 ⟩ -->* (to_redex (inl [v2])))
+  \/  (exists q2,
+          r = inr q2
+      /\  ⟨ [], e2 ⟩ -->* (to_redex (inr q2))))
+  ->  ⟨ [], °(ECons e1 e2) ⟩ -->* (to_redex r).
+Proof.
+  itr.
+  des - H as [H | [H | H]].
+  * des - H as [v1 [v2 [Heq [Hv1 Hv2]]]].
+    sbt.
+    des - Hv1 as [k1 [Hscope1 Hstep1]].
+    des - Hv2 as [k2 [Hscope2 Hstep2]].
+    open / Hscope1 Hscope2.
+    step - Hstep2.
+    step - Hstep1.
+    step.
+  * des - H as [v1 [v2 [Heq [Hv1 Hv2]]]].
+    sbt.
+    des - Hv1 as [k1 [Hscope1 Hstep1]].
+    des - Hv2 as [k2 [Hscope2 Hstep2]].
+    open / Hscope1 Hscope2.
+    step - Hstep2.
+    step - Hstep1.
+    step.
+  * des - H as [v2 [Heq Hv2]].
+    sbt.
+    des - Hv2 as [k2 [Hscope2 Hstep2]].
+    open / Hscope2.
+    step - Hstep2.
+    step.
+Qed.
+
+Theorem exi_nat_plus :
+  forall n,
+    exists n1 n2,
+      n = n1 + n2.
+Proof.
+  ind - n.
+  exi - 0 0.
+  trv.
+  des - IHn as [n1 [n2 IHn]].
+  exi - (S n1) n2.
+  rwr - Nat.add_succ_l.
+  bwr - IHn.
+Qed.
+
+Theorem trans_middle :
+  forall k Fs1 Fs3 e1 e3,
+      ⟨ Fs1, e1 ⟩ -[k]-> ⟨ Fs3, e3 ⟩
+  ->  exists k1 k2 Fs2 e2,
+          ⟨ Fs1, e1 ⟩ -[k1]-> ⟨ Fs2, e2 ⟩
+      /\  ⟨ Fs2, e2 ⟩ -[k2]-> ⟨ Fs3, e3 ⟩.
+Proof.
+  itr.
+  induction H.
+  * exi - 0 0 fs e.
+    spl.
+    cns.
+    cns.
+  * (* pse - exi_nat_plus: k.
+    des - H1 as [k1 [k2 Heqk]].
+    sbt. *)
+    des - IHstep_rt as [k1 [k2 [Fs2 [e2 [Hstep1 Hstep2]]]]].
+    exi - (S k1) k2 Fs2 e2.
+    spl.
+    2: asm.
+    ens.
+    exa - H.
+    asm.
+Qed.
+
+
+
+Theorem split_econs_first :
+  forall e1 e2 vs,
+    ⟨ [], °(ECons e1 e2) ⟩ -->* (RValSeq vs)
+  ->  exists v2,
+      ⟨ [], RExp e2 ⟩ -->* (RValSeq [v2]).
+Proof.
+  itr.
+  ivc - H as [k [Hscope Hstep]].
+  pse - trans_middle:
+        k ([] : FrameStack) ([] : FrameStack)
+        (°(ECons e1 e2)) (RValSeq vs)
+        Hstep.
+  des - H as [k1 [k2 [Fs [e [Hstep1 Hstep2]]]]].
+  ivs - Hstep1.
+  * ivs - Hstep2.
+    ivc - H.
+    clr + H0.
+    ivs - H0.
+    ivs - H1.
+    - ivs - H0.
+      ivs - H6.
+      ivs - H3.
+    - ivs - H.
+Admitted.
+    
+
+
+
+Lemma destruct_econs2 :
+  forall e1 e2 r,
+      ⟨ [], °(ECons e1 e2) ⟩ -->* (to_redex r)
+  ->  (exists v1 v2,
+          r = inl [VCons v1 v2]
+      /\  ⟨ [], RExp e1 ⟩ -->* (to_redex (inl [v1]))
+      /\  ⟨ [], RExp e2 ⟩ -->* (to_redex (inl [v2])))
+  \/  (exists q1 v2,
+          r = inr q1
+      /\  ⟨ [], RExp e1 ⟩ -->* (to_redex (inr q1))
+      /\  ⟨ [], RExp e2 ⟩ -->* (to_redex (inl [v2])))
+  \/  (exists q2,
+          r = inr q2
+      /\  ⟨ [], RExp e2 ⟩ -->* (to_redex (inr q2))).
+Proof.
+  itr.
+  ivc - H as [k [Hscope Hstep]].
+  eapply transitive_eval in Hstep.
+  ivc - Hstep.
+  des - r; ivc - H2.
+  ivs - H.
+  eapply transitive_eval_rev in H0.
+  ivs - H0.
+  ivs - H1.
+  des - r as [vs | q]; smp *.
+  * lft.
+    ivc - H as [k [_ H1]].
+    ivc - H1.
+    ivc - H.
+    ivc - H0.
+    ivc - H.
+    2: {
+    trv.
+    ivc - H.
+  * ivc - H as [k [_ H1]].
+    ivc - H1.
+    ivc - H.
+    ivc - H0.
+    ivc - H.
+Qed.
+
+
+
+
+
+
+
+
+
+
+
+
+
+Theorem eq_fsbs :
+  forall e r,
+      step_any [] (RExp e) (to_redex r)
+  ->  eval_expr_simpl (give_names e) (give_result r).
+Proof.
+  ind ~ ind_fs_exp - e;
+        itr - r HF.
+  (* VNil*)
+  14:{
+    app - destruct_value in HF.
+    sbt.
+    app - value_to_value.
+  }
+  3: {
+    app - destruct_econs in HF.
+  }
+Admitted.
+
+
+
+
+
+
+
+
+
+
+
+
+
+
+
+
+
+
+
+
+
+
+
+
+
+
+
+
+
+
+
+
+
+
+
+
+(* Definition result_in_scope
+    ()
+
+Axiom result_scope :
+    forall r,
+    to_redex. *)
+
+Fixpoint no_reference_val
+    (v : Val)
+    : Prop
+    :=
+  match v with
+
+  | VNil => True
+
+  | VLit _ => True
+
+  | VVar _ => False
+
+  | VFunId _ => False
+
+  | VPid _ => False
+
+  | VCons v1 v2 => no_reference_val v1 /\ no_reference_val v2
+
+  | VTuple vs =>
+    fold_right
+        (fun v acc =>
+          no_reference_val v /\ acc)
+        True
+        vs
+
+  | VMap vvs =>
+    fold_right
+        (fun '(vk, vv) acc =>
+          no_reference_val vk /\ no_reference_val vv /\ acc)
+        True
+        vvs
+
+  | VClos _ _ _ _ => True
+
+  end.
+
+Import BigStep.
+
+Fixpoint no_reference_exp
+    (e : Expression)
+    : Prop
+    :=
+  match e with
+
+  | ENil => True
+
+  | ELit _ => True
+
+  | EVar _ => False
+
+  | EFunId _ => False
+
+  | ECons e1 e2 => no_reference_exp e1 /\ no_reference_exp e2
+
+  | ESeq e1 e2 => no_reference_exp e1 /\ no_reference_exp e2
+
+  | ETuple es =>
+    fold_right
+        (fun e acc =>
+          no_reference_exp e /\ acc)
+        True
+        es
+
+  | EValues es =>
+    fold_right
+        (fun e acc =>
+          no_reference_exp e /\ acc)
+        True
+        es
+
+  | EPrimOp _ es =>
+    fold_right
+        (fun e acc =>
+          no_reference_exp e /\ acc)
+        True
+        es
+
+  | EApp e es =>
+    no_reference_exp e /\
+    fold_right
+        (fun e acc =>
+          no_reference_exp e /\ acc)
+        True
+        es
+
+  | ECall em ef es =>
+    no_reference_exp em /\
+    no_reference_exp ef /\
+    fold_right
+        (fun e acc =>
+          no_reference_exp e /\ acc)
+        True
+        es
+
+  | EMap ees =>
+    fold_right
+        (fun '(ek, ev) acc =>
+          no_reference_exp ek /\ no_reference_exp ev /\ acc)
+        True
+        ees
+
+  | _ => True
+
+  end.
+
+
+
+Theorem eval_value_no_reference :
+  forall v r,
+      ⟨ [], ˝v ⟩ -->* r
+  ->  no_reference_val v.
+Proof.
+  itr.
+  ind ~ ind_fs_val - v; smp; trv.
+  * admit.
+  * ivc - H as [k [H1 H2]].
+    ivc - H2.
+    ivc - H1.
+    ivc - H.
+    ivc - H4.
+    ivc - H3.
+  * ivc - H as [k [H1 H2]].
+    ivc - H2.
+    ivc - H1.
+    ivc - H.
+    ivc - H4.
+    ivc - H3.
+  * 
+  
+    unfold is_result in H1.
+    1: con.
+
+
 
 Lemma any_cool_value :
   forall v,
